sketching adequacy

fairness/heap_lang/simulation_adequacy.v
@@ -1,8 +1,10 @@
 From stdpp Require Import fin_maps.
 From iris.proofmode Require Import tactics.
 From trillium.program_logic Require Export weakestpre adequacy.
+From trillium.fairness Require Export fairness.
 From trillium.fairness.heap_lang Require Export lang heap_lang_defs.
 
+Definition heap_lang_extrace : Type := extrace heap_lang.
 
 Section adequacy.
 (* Context . *)
