fairness/lawyer/eo_fin_adequacy.v
@@ -1,15 +1,117 @@
+From iris.algebra Require Import auth gmap gset excl excl_auth.
 From trillium.fairness.heap_lang Require Import simulation_adequacy.
-From trillium.fairness.lawyer Require Import obligations_model.
+From trillium.fairness.lawyer Require Import obligations_model obligations_resources.
+From trillium.fairness.lawyer Require Import eo_fin. 
+
+
+Section OMTermination.
+  Context `(OP: ObligationsParams Degree Level Locale LIM_STEPS).
+  Context `{Countable Locale}. 
+  Let OM := ObligationsModel OP. 
+
+  Definition has_obls (τ: Locale) (s: mstate OM) := default ∅ (ps_obls _ s !! τ) ≠ ∅. 
+
+  Definition obls_trace_fair := fair_by has_obls eq.
+
+  Definition obls_trace_valid := trace_valid (@mtrans OM).
+
+  Definition obls_trace := trace (mstate OM) (mlabel OM). 
+
+  Lemma obls_fair_trace_terminate (tr: obls_trace):
+    obls_trace_valid tr ->
+    (∀ τ, obls_trace_fair τ tr) ->
+    terminating_trace tr.
+  Proof. Admitted. 
+
+End OMTermination.
 
 
 Section ObligationsAdequacy.
 
-  Context {Λ: language}. 
-  Context `(OP: ObligationsParams Degree Level (locale Λ) LIM_STEPS).
-  Context `{Countable (locale Λ)}.
+  Context {DegO LevelO: ofe}.
+  Context `{OfeDiscrete DegO} `{OfeDiscrete LevelO} `{@LeibnizEquiv (ofe_car LevelO) (ofe_equiv LevelO)}.
+  Context {LIM_STEPS: nat}.
+
+  Let Degree := ofe_car DegO.
+  Let Level := ofe_car LevelO.
+
+  Context (OP: ObligationsParams Degree Level (locale heap_lang) LIM_STEPS).
   Let OM := ObligationsModel OP.
 
-  
-  
+  (* Context `{hGS: @heapGS Σ _ EM}. *)
+  (* Let oGS : ObligationsGS EO_OP Σ := heap_fairnessGS (heapGS := hGS). *)
+
+  Let EM := @ObligationsEM DegO LevelO _ _ _ heap_lang _ _ _ OP.
+
+  Theorem simple_simulation_adequacy_terminate_ftm Σ 
+
+    `{FairTerminatingModelSimple M}
+
+        `{!heapGpreS Σ (@LM_EM_HL _ _ _ LF)} (s: stuckness)
+        e1 (s1: M) FR
+        (LSI0: initial_ls_LSI s1 0)
+        (extr : heap_lang_extrace)
+        (Hexfirst : (trfirst extr).1 = [e1])
+    :
+    (* The model has finite branching *)
+    rel_finitary (sim_rel LM) →
+    wp_premise (λ _ _, True) (trfirst extr).2 e1 s1 s FR LSI0 -> 
+    (* The coinductive pure coq proposition given by adequacy *)
+    extrace_fairly_terminating extr.
+  Proof.
+    intros. eapply simulation_adequacy_terminate =>//.
+    intros ? _.
+    by eapply simple_fair_terminating_traces_terminate.
+  Qed.
+
+
 
 End ObligationsAdequacy.
+
+
+Section EOFinAdequacy.
+
+  Context (LIM: nat). 
+
+  Let EM := EO_EM LIM.
+
+  Let eofinΣ: gFunctors := #[
+      GFunctor (excl_authR natO); 
+      GFunctor (authUR (gmapUR nat (agreeR SignalId)));
+      heapΣ EM
+].
+
+  Global Instance subG_eofinΣ {Σ}: subG eofinΣ Σ → EoFinPreG Σ.
+  Proof. solve_inG. Qed.
+
+  Theorem eofin_terminates
+    (N : nat)
+    (HN: N > 1)
+    (extr : heap_lang_extrace)
+    (Hvex : extrace_valid extr)
+    (Hexfirst : (trfirst extr).1 = [start #N]):
+    (∀ tid, fair_ex tid extr) -> terminating_trace extr.
+  Proof.
+    assert (heapGpreS eofinΣ EM) as HPreG.
+    { apply _. }
+    eapply (simulation_adequacy_terminate_ftm yesnoΣ the_model NotStuck _ (N, true) ∅) =>//.
+    - eapply valid_state_evolution_finitary_fairness_simple.
+      intros ?. simpl. apply (model_finitary s1).
+    - intros ?. iStartProof. iIntros "!> (Hm & HFR & Hf) !>". simpl.
+      
+      iApply (start_spec _ _ 61 with "[Hm Hf HFR]"); eauto.
+      
+      + iSplitL "Hm"; eauto. do 2 (destruct N; first lia).
+        iFrame. iSplit; last (iPureIntro; lia).
+        assert ({[Y := 61%nat; No := 61%nat]} = gset_to_gmap 61 {[No;Y]}) as <-; last done.
+        rewrite -leibniz_equiv_iff. intros ρ.
+        destruct (gset_to_gmap 61 {[Y; No]} !! ρ) as [f|] eqn:Heq.
+        * apply lookup_gset_to_gmap_Some in Heq as [Heq ->].
+          destruct (decide (ρ = Y)) as [-> |].
+          ** rewrite lookup_insert //. rewrite lookup_gset_to_gmap option_guard_True //. set_solver.
+          ** rewrite lookup_insert_ne //. assert (ρ = No) as -> by set_solver.
+             rewrite lookup_insert // lookup_gset_to_gmap option_guard_True //. set_solver.
+        * apply lookup_gset_to_gmap_None in Heq. destruct ρ; set_solver.
+  Qed.  
+
+End EOFinAdequacy.
